Work in progress on doing generalized term compilation

ffi/ByteStringFFI.v
@@ -4,6 +4,7 @@ Require Import
   ByteString.Lib.Fiat
   ByteString.Lib.TupleEnsembles
   ByteString.Lib.FunMaps
+  ByteString.Lib.FromADT
   ByteString.Memory
   ByteString.Heap
   ByteString.FFI.HeapFFI
@@ -26,60 +27,64 @@ Import Heap.
 Import HeapState.
 Import FMapExt.
 
-Inductive HeapF (r : Type) : Type :=
-  | Alloc   : forall (len : Size | 0 < len) (k : N -> r), HeapF r
-  | Free_   : forall (addr : Ptr Word), r -> HeapF r
-  | Realloc : forall (addr : Ptr Word) (len : Size | 0 < len) (k : N -> r), HeapF r
-  | Peek    : forall (addr : Ptr Word) (k : Word -> r), HeapF r
-  | Poke    : forall (addr : Ptr Word) (w : Word), r -> HeapF r
-  | Memcpy  : forall (addr : Ptr Word) (addr2 : Ptr Word) (len : Size), r -> HeapF r
-  | Memset  : forall (addr : Ptr Word) (len : Ptr Word) (w : Word), r -> HeapF r.
+Inductive callArgs (r : Type) : list Type -> option Type -> Type :=
+  | RetVal  : r -> callArgs r [] None
+  | ContVal : forall cod, (cod -> r) -> callArgs r [] (Some cod)
+  | ArgVal  : forall t ts cod, t -> callArgs r ts cod
+                -> callArgs r (t :: ts) cod.
 
-Program Instance HeapF_Functor : Functor HeapF := {
-  fmap := fun _ _ f x =>
-    match x with
-    | Alloc len k             => Alloc len (compose f k)
-    | Free_ addr x            => Free_ addr (f x)
-    | Realloc addr len k      => Realloc addr len (compose f k)
-    | Peek addr k             => Peek addr (compose f k)
-    | Poke addr w x           => Poke addr w (f x)
-    | Memcpy addr addr2 len x => Memcpy addr addr2 len (f x)
-    | Memset addr len w x     => Memset addr len w (f x)
-    end
+Program Instance callArgs_Functor (dom : list Type) (cod : option Type) :
+  Functor (fun r => callArgs r dom cod) := {
+  fmap := fun A B f x =>
+            let fix go dom cod (z : callArgs A dom cod) :=
+                match z with
+                | RetVal x          => RetVal (f x)
+                | ContVal _ k       => ContVal (f \o k)
+                | ArgVal _ _ _ x xs => ArgVal x (go _ _ xs)
+                end in
+            go _ _ x
 }.
 
-Definition HeapDSL := Free HeapF.
+Inductive methodCall (sig : ADTSig) (adt : ADT sig) (rec : Type) : Type :=
+  | Call : forall (midx : MethodIndex sig)
+                  (args : callArgs rec (fst (MethodDomCod sig midx))
+                                       (snd (MethodDomCod sig midx))),
+      methodCall adt rec.
 
-Inductive HeapF_Computes :
-  forall {A}, HeapF A -> Rep HeapSpec -> Rep HeapSpec -> A -> Prop :=
-  | HAlloc len addr (r r' : Rep HeapSpec) A (k : Ptr Word -> A) x :
-      alloc r len ↝ (r', addr) ->
-      x = k addr ->
-      HeapF_Computes (Alloc len k) r r' x
+Program Instance methodCall_Functor (sig : ADTSig) (adt : ADT sig) :
+  Functor (methodCall adt) := {
+  fmap := fun A B f x =>
+            match x with
+            | Call midx args => Call adt midx (fmap f args)
+            end
+}.
 
-  | HFree addr (r r' : Rep HeapSpec) A (x : A) :
-      free r addr ↝ (r', tt) ->
-      HeapF_Computes (Free_ addr x) r r' x
+Definition CallDSL (sig : ADTSig) (adt : ADT sig) : Type -> Type :=
+  Free (methodCall adt).
 
-  | HRealloc addr len addr' (r r' : Rep HeapSpec) A (k : Ptr Word -> A) :
-      realloc r addr len ↝ (r', addr') ->
-      HeapF_Computes (Realloc addr len k) r r' (k addr')
+Inductive call_represented (sig : ADTSig) (adt : ADT sig) :
+          forall (dom : list Type) (cod : option Type) A,
+            callArgs A dom cod -> methodType' (Rep adt) dom cod -> A -> Prop :=
+  | CheckRet : forall A (v : A) (meth : methodType' (Rep adt) [] None),
+      call_represented adt (RetVal v) meth v
+  | CheckCont : forall cod A (k : cod -> A) (x : cod)
+                       (meth : methodType' (Rep adt) [] (Some cod)) v,
+      v = k x -> call_represented adt (ContVal k) meth v
+  | CheckArg : forall t ts (x : t) (cod : option Type) A
+                      (args : callArgs A ts cod)
+                      (meth : methodType' (Rep adt) (t :: ts) cod) v,
+      call_represented adt args (meth x) v ->
+      call_represented adt (ArgVal x args) meth v.
 
-  | HPeek addr w (r r' : Rep HeapSpec) A (k : Word -> A) :
-      peek r addr ↝ (r', w) ->
-      HeapF_Computes (Peek addr k) r r' (k w)
-
-  | HPoke addr w (r r' : Rep HeapSpec) A (x : A) :
-      poke r addr w ↝ (r', tt) ->
-      HeapF_Computes (Poke addr w x) r r' x
-
-  | HMemcpy addr addr2 len r r' A (x : A) :
-      memcpy r addr addr2 len ↝ (r', tt) ->
-      HeapF_Computes (Memcpy addr addr2 len x) r r' x
-
-  | HMemset addr len w r r' A (x : A) :
-      memset r addr len w ↝ (r', tt) ->
-      HeapF_Computes (Memset addr len w x) r r' x.
+Inductive methodCall_Computes (sig : ADTSig) (adt : ADT sig) :
+  forall A, methodCall adt A -> Rep adt -> Rep adt -> A -> Prop :=
+  | CallComputes (midx : MethodIndex sig) A
+                 (args : callArgs A (fst (MethodDomCod sig midx))
+                                    (snd (MethodDomCod sig midx)))
+                 (r r' : Rep adt) v :
+      fromMethod (Methods adt midx) r r'
+        -> call_represented adt args (Methods adt midx r) v
+        -> methodCall_Computes (Call adt midx args) r r' v.
 
 Inductive Free_Computes `{Functor f} {R : Type}
           (crel : forall {A}, f A -> R -> R -> A -> Prop) :
@@ -91,44 +96,50 @@ Inductive Free_Computes `{Functor f} {R : Type}
         -> crel A t r r' v
         -> Free_Computes crel (Join k t) r r'' v'.
 
-Definition HeapDSL_Computes `(h : HeapDSL A) :=
-  Free_Computes (@HeapF_Computes) h.
+Definition ADT_Computes (sig : ADTSig) (adt : ADT sig)
+           `(r : CallDSL adt A) :=
+  Free_Computes (@methodCall_Computes sig adt) r.
 
 Definition ByteString (r : Rep HeapSpec) := Rep (projT1 (ByteStringHeap r)).
 
-Definition reflect_Heap_DSL_computation {A : Type}
-           (c : Rep HeapSpec * PS -> Comp ((Rep HeapSpec * PS) * A)) :=
-  { f : PS -> HeapDSL (PS * A)
-  & forall r bs r' bs' v, c (r, bs) ↝ ((r', bs'), v)
-      -> HeapDSL_Computes (f bs) r r' (bs', v) }.
+Section Reflection.
 
-Lemma reflect_computation_ret {A : Type} (v : A) :
-  reflect_Heap_DSL_computation (fun r => ret (r, v)).
+Variable sig : ADTSig.
+Variable adt : ADT sig.
+
+Definition reflect_ADT_DSL_computation {A B : Type}
+           (c : Rep adt * B -> Comp ((Rep adt * B) * A)) :=
+  { f : B -> CallDSL adt (B * A)
+  & forall r bs r' bs' v, c (r, bs) ↝ ((r', bs'), v)
+      -> ADT_Computes (f bs) r r' (bs', v) }.
+
+Lemma reflect_computation_ret {A B : Type} (v : A) :
+  reflect_ADT_DSL_computation (B:=B) (fun r => ret (r, v)).
 Proof.
   exists (fun r => pure (r, v)); intros.
   computes_to_inv; injections.
   eapply CPure.
 Defined.
 
-Lemma reflect_Heap_DSL_computation_simplify {B : Type} c c'
+Lemma reflect_ADT_DSL_computation_simplify {B C : Type} c c'
       (refine_c_c' : forall r, refineEquiv (c r) (c' r))
-      (c_DSL : reflect_Heap_DSL_computation c')
-  : reflect_Heap_DSL_computation (A := B) c.
+      (c_DSL : reflect_ADT_DSL_computation c')
+  : reflect_ADT_DSL_computation (A := C) (B := B) c.
 Proof.
   exists (projT1 c_DSL); intros.
   pose proof (projT2 c_DSL); simpl in *.
   apply H0; apply refine_c_c'; auto.
 Defined.
 
-Lemma reflect_Heap_DSL_computation_If_Then_Else
-      {B : Type} c c' (t e : _ -> Comp (_ * B))
-      (c_DSL : reflect_Heap_DSL_computation t)
-      (k_DSL : reflect_Heap_DSL_computation e)
+Lemma reflect_ADT_DSL_computation_If_Then_Else
+      {B C : Type} c c' (t e : _ -> Comp (_ * C))
+      (c_DSL : reflect_ADT_DSL_computation t)
+      (k_DSL : reflect_ADT_DSL_computation e)
   : (forall r, c r = c' (snd r)) ->
-    reflect_Heap_DSL_computation (fun r => If c r Then t r Else e r).
+    reflect_ADT_DSL_computation (B:=B) (fun r => If c r Then t r Else e r).
 Proof.
   intros.
-  exists (fun bs : PS =>
+  exists (fun bs : B =>
             If c' bs
             Then projT1 c_DSL bs
             Else projT1 k_DSL bs).
@@ -139,11 +150,13 @@ Proof.
   destruct (c' _).
     destruct c_DSL.
     simpl in *.
-    apply h; assumption.
+    apply a; assumption.
   destruct k_DSL.
   simpl in *.
-  apply h; assumption.
+  apply a; assumption.
 Defined.
+
+End Reflection.
 
 Hint Unfold id.
 Hint Unfold bind.
@@ -158,32 +171,46 @@ Hint Unfold poke_at_offset.
 Hint Unfold buffer_cons.
 
 Ltac simplify_reflection :=
-  eapply reflect_Heap_DSL_computation_simplify;
+  eapply reflect_ADT_DSL_computation_simplify;
   [ set_evars; intros;
     autorewrite with monad laws; simpl;
     try rewrite refineEquiv_If_Then_Else_Bind;
     finish honing
-  | try (eapply reflect_Heap_DSL_computation_If_Then_Else;
+  | try (eapply reflect_ADT_DSL_computation_If_Then_Else;
          [| | let r := fresh "r" in
               intro r; destruct r; simpl; reflexivity]) ].
 
-Ltac prepare_reflection :=
-  repeat match goal with
-  | [ |- reflect_Heap_DSL_computation _ ] =>
-    eexists; intros; try computes_to_inv; tsubst
-  | [ H : _ * _ |- _ ] => destruct H
-  | [ H : () |- _ ] => destruct H
-  end; simpl in *.
-
 Ltac DSL_term :=
   repeat match goal with
-    [ H : _ ↝ (?R, _) |- HeapF_Computes _ _ ?R _ ] =>
+    [ H : _ ↝ (?R, _) |- methodCall_Computes _ _ ?R _ ] =>
     solve [ econstructor; eassumption
           | econstructor; [eassumption|higher_order_reflexivity] ]
   end.
 
+Ltac build_computational_spine :=
+  repeat match goal with
+  | [ |- reflect_ADT_DSL_computation _ _ ] => eexists; intros
+  (* | H : {a' | @?P a'} ↝ _ |- _ => apply Pick_inv in H *)
+  (* | H : Return ?a ↝ _ |- _ => *)
+  (*   apply Return_inv in H; tsubst; try apply CPure *)
+  (* | H : Bind (A := ?A) ?ca ?k ↝ _ |- _ => *)
+  (*   apply Bind_inv in H; *)
+  (*   let a' := fresh "v" in *)
+  (*   let H' := fresh H "'" in *)
+  (*   destruct H as [a' [H H'] ]; *)
+  (*   eapply CJoin *)
+  end;
+  computes_to_inv; tsubst; simpl in *;
+  repeat match goal with
+  | [ H : _ * _ |- _ ] => destruct H
+  | [ H : () |- _ ] => destruct H
+  end.
+
+Lemma lt_0_n : forall n, 0 < n + 1.
+Proof. nomega. Qed.
+
 Definition consDSL w :
-  reflect_Heap_DSL_computation
+  reflect_ADT_DSL_computation HeapSpec
     (fun r => r' <- buffer_cons (fst r) (snd r) w; ret (r', ()))%comp.
 Proof.
   Local Opaque poke.
@@ -196,73 +223,158 @@ Proof.
 
   simplify_reflection.
     simplify_reflection.
-    prepare_reflection.
-    eapply CJoin.
-      apply CPure.
-    DSL_term.
+    { build_computational_spine.
+
+      eapply CJoin.
+      eapply CPure.
+
+      apply CallComputes (* poke *)
+        with (midx := Fin.FS (Fin.FS (Fin.FS (Fin.FS Fin.F1)))).
+        repeat eexists; eassumption.
+      apply CheckArg with (x := psBuffer bs + (psOffset bs - 1)).
+      apply CheckArg with (x := w).
+      eapply CheckCont; higher_order_reflexivity.
+    }
 
   simplify_reflection.
     simplify_reflection.
-    prepare_reflection.
-    eapply CJoin.
+    { build_computational_spine.
+
       eapply CJoin.
-        eapply CPure.
-      DSL_term.
-    DSL_term.
+      eapply CJoin.
+      eapply CPure.
+
+      apply CallComputes (* poke *)
+        with (midx := Fin.FS (Fin.FS (Fin.FS (Fin.FS Fin.F1)))).
+        repeat eexists; eassumption.
+      apply CheckArg with (x := psBuffer bs + 0).
+      apply CheckArg with (x := w).
+      eapply CheckCont; higher_order_reflexivity.
+
+      apply CallComputes (* memcpy *)
+        with (midx := Fin.FS (Fin.FS (Fin.FS (Fin.FS (Fin.FS Fin.F1))))).
+        repeat eexists; eassumption.
+      apply CheckArg with (x := psBuffer bs).
+      apply CheckArg with (x := psBuffer bs + 1).
+      apply CheckArg with (x := psLength bs).
+      eapply CheckCont; higher_order_reflexivity.
+    }
 
   simplify_reflection.
     simplify_reflection.
-    prepare_reflection.
-    eapply CJoin.
+    { build_computational_spine.
+
       eapply CJoin.
-        eapply CJoin.
-          eapply CJoin.
-            eapply CPure.
-          DSL_term.
-        DSL_term.
-      DSL_term.
-    DSL_term.
+      eapply CJoin.
+      eapply CJoin.
+      eapply CJoin.
+      eapply CPure.
+
+      apply CallComputes (* poke *)
+        with (midx := Fin.FS (Fin.FS (Fin.FS (Fin.FS Fin.F1)))).
+        repeat eexists; eassumption.
+      apply CheckArg with (x := p + 0).
+      apply CheckArg with (x := w).
+      eapply CheckCont; higher_order_reflexivity.
+
+      apply CallComputes (* free *)
+        with (midx := Fin.FS Fin.F1).
+        repeat eexists; eassumption.
+      apply CheckArg with (x := psBuffer bs).
+      eapply CheckCont; higher_order_reflexivity.
+
+      apply CallComputes (* memcpy *)
+        with (midx := Fin.FS (Fin.FS (Fin.FS (Fin.FS (Fin.FS Fin.F1))))).
+        repeat eexists; eassumption.
+      apply CheckArg with (x := psBuffer bs).
+      apply CheckArg with (x := p + 1).
+      apply CheckArg with (x := psLength bs).
+      eapply CheckCont; higher_order_reflexivity.
+
+      simpl in *.
+      apply CallComputes (* alloc *)
+        with (midx := Fin.F1).
+        do 2 eexists; eassumption.
+      apply CheckArg with (x := exist _ (psLength bs + 1) (lt_0_n _)).
+      apply CheckCont with (x := p); higher_order_reflexivity.
+    }
 
   simplify_reflection.
-  prepare_reflection.
-  eapply CJoin.
-    eapply CJoin.
-      apply CPure.
-    DSL_term.
-  DSL_term.
+    { build_computational_spine.
+
+      eapply CJoin.
+      eapply CJoin.
+      eapply CPure.
+
+      apply CallComputes (* poke *)
+        with (midx := Fin.FS (Fin.FS (Fin.FS (Fin.FS Fin.F1)))).
+        repeat eexists; eassumption.
+      apply CheckArg with (x := p + 0).
+      apply CheckArg with (x := w).
+      eapply CheckCont; higher_order_reflexivity.
+
+      simpl in *.
+      apply CallComputes (* alloc *)
+        with (midx := Fin.F1).
+        do 2 eexists; eassumption.
+      apply CheckArg with (x := exist _ _ N.lt_0_1).
+      apply CheckCont with (x := p); higher_order_reflexivity.
+    }
+
+  Local Transparent poke.
+  Local Transparent alloc.
+  Local Transparent free.
+  Local Transparent peek.
+  Local Transparent memcpy.
+
+  Unshelve.
+  all: exact tt.
 Defined.
 
-Definition denote {A : Type} :
-  HeapDSL A -> Rep HeapSpec -> Comp (Rep HeapSpec * A) :=
-  let phi (c : HeapF (Rep HeapSpec -> Comp (Rep HeapSpec * A))) := fun r =>
-    match c with
-    | Alloc len k             => `(r', addr) <- alloc r len; k addr r'
-    | Free_ addr x            => `(r', _)    <- free r addr; x r'
-    | Realloc addr len k      => `(r', addr) <- realloc r addr len; k addr r'
-    | Peek addr k             => `(r', w)    <- peek r addr; k w r'
-    | Poke addr w x           => `(r', _)    <- poke r addr w; x r'
-    | Memcpy addr addr2 len x => `(r', _)    <- memcpy r addr addr2 len; x r'
-    | Memset addr len w x     => `(r', _)    <- memset r addr len w; x r'
+Definition consDSL' w := Eval simpl in projT1 (consDSL w).
+Print consDSL'.
+
+Definition applyArgs
+           (dom : list Type) (cod : option Type)
+           {rep : Type} (meth : methodType rep dom cod)
+           {A : Type} (args : callArgs A dom cod) :
+  rep -> Comp (rep * A).
+Proof.
+  intro r.
+  induction dom.
+    destruct cod; inv args.
+      exact (`(r', t) <- meth r; ret (r', X t)).
+    exact (r' <- meth r; ret (r', X))%comp.
+  inv args.
+  exact (IHdom (fun r => meth r X) X0).
+Defined.
+
+Definition denote (sig : ADTSig) (adt : ADT sig) {A : Type} :
+  CallDSL adt A -> Rep adt -> Comp (Rep adt * A) :=
+  let phi (c : methodCall adt (Rep adt -> Comp (Rep adt * A))) :=
+    match c return Rep adt -> Comp (Rep adt * A) with
+    | Call midx args => fun r =>
+        `(r', k) <- applyArgs (rep:=Rep adt) (Methods adt midx) args r; k r'
     end in
   iter phi \o fmap (fun x r => ret (r, x)).
 
-Corollary denote_Pure : forall A (x : A) r,
-  refineEquiv (denote (Pure x) r) (ret (r, x)).
+Corollary denote_Pure (sig : ADTSig) (adt : ADT sig) : forall A (x : A) r,
+  refineEquiv (denote (adt:=adt) (Pure x) r) (ret (r, x)).
 Proof. reflexivity. Qed.
 
-Lemma denote_Join : forall A B (k : A -> HeapDSL B) (h : HeapF A) r,
+Lemma denote_Join (sig : ADTSig) (adt : ADT sig) :
+  forall A B (k : A -> CallDSL adt B) (h : methodCall adt A) r,
   refineEquiv (denote (Join k h) r)
               (denote (liftF h) r >>= fun p => denote (k (snd p)) (fst p)).
 Proof.
   intros.
-  unfold denote, iter; simpl.
-  induction h;
-  autorewrite with monad laws; reflexivity.
-Qed.
+  destruct h.
+Admitted.
 
-Lemma denote_Free_bind : forall A (x : HeapDSL A) B (k : A -> HeapDSL B) r,
-  refineEquiv (denote (Free_bind k x) r)
-              (denote x r >>= fun p => denote (k (snd p)) (fst p)).
+Lemma denote_Free_bind (sig : ADTSig) (adt : ADT sig) :
+  forall A (x : CallDSL adt A) B (k : A -> CallDSL adt B) r,
+    refineEquiv (denote (Free_bind k x) r)
+                (denote x r >>= fun p => denote (k (snd p)) (fst p)).
 Proof.
   intros.
   generalize dependent r.
@@ -277,13 +389,15 @@ Proof.
   reflexivity.
 Qed.
 
-Corollary denote_If : forall b A (t e : HeapDSL A) r,
-  refineEquiv (denote (If b Then t Else e) r)
-              (If b Then denote t r Else denote e r).
+Corollary denote_If (sig : ADTSig) (adt : ADT sig) :
+  forall b A (t e : CallDSL adt A) r,
+    refineEquiv (denote (If b Then t Else e) r)
+                (If b Then denote t r Else denote e r).
 Proof. destruct b; simpl; reflexivity. Qed.
 
-Lemma HeapDSL_Computes_denotation : forall A f r r' (v : A),
-  denote f r ↝ (r', v) -> HeapDSL_Computes f r r' v.
+Lemma ADT_Computes_denotation (sig : ADTSig) (adt : ADT sig) :
+  forall A f r r' (v : A),
+    denote f r ↝ (r', v) -> ADT_Computes (adt:=adt) f r r' v.
 Proof.
   intros.
   generalize dependent r.
@@ -303,15 +417,112 @@ Proof.
   destruct v0;
   eapply CJoin;
   simpl in H0';
-  [ apply H; eauto | eapply HAlloc
-  | apply H; eauto | apply HFree
-  | apply H; eauto | apply HRealloc
-  | apply H; eauto | apply HPeek
-  | apply H; eauto | apply HPoke
-  | apply H; eauto | apply HMemcpy
-  | apply H; eauto | apply HMemset ];
+  [ apply H; eauto | eapply CallComputes ];
   try destruct u; eauto.
-Qed.
+Admitted.
+
+Axiom IO : Type -> Type.
+
+Axiom fmapIO   : forall {a b : Type}, (a -> b) -> IO a -> IO b.
+Axiom bindIO   : forall {a b : Type}, IO a -> (a -> IO b) -> IO b.
+Axiom returnIO : forall {a : Type}, a -> IO a.
+Axiom failIO   : forall {a : Type}, IO a.
+Axiom joinIO   : forall {a : Type}, IO (IO a) -> IO a.
+
+Axiom bindIO_returnIO : forall {a b : Type} (f : a -> b) (x : IO a),
+  bindIO x (fun a => returnIO (f a)) = fmapIO f x.
+
+Axiom unsafeDupablePerformIO : forall {a : Type}, IO a -> a.
+
+Axiom malloc  : Size -> IO (Ptr Word).
+Axiom free    : Ptr Word -> IO ().
+Axiom realloc : Ptr Word -> Size -> IO (Ptr Word).
+Axiom peek    : Ptr Word -> IO Word.
+Axiom poke    : Ptr Word -> Word -> IO ().
+Axiom memcpy  : Ptr Word -> Ptr Word -> Size -> IO ().
+Axiom memset  : Ptr Word -> Size -> Word -> IO ().
+
+Definition ghcDenote {A : Type} : CallDSL HeapSpec A -> A.
+Proof.
+  intros.
+  apply (fmap returnIO) in X.
+  eapply (iter _) in X.
+  apply unsafeDupablePerformIO in X.
+  exact X.
+  Unshelve.
+  clear X.
+  destruct 1.
+  simpl in *.
+  dependent destruction midx; simpl in *.
+    inv args. inv X0.
+    exact (bindIO (malloc (` X)) X1).
+  dependent destruction midx; simpl in *.
+    inv args. inv X0.
+    exact (bindIO (free X) X1).
+  dependent destruction midx; simpl in *.
+    inv args. inv X0. inv X2.
+    exact (bindIO (realloc X (` X1)) X0).
+  dependent destruction midx; simpl in *.
+    inv args. inv X0.
+    exact (bindIO (peek X) X1).
+  dependent destruction midx; simpl in *.
+    inv args. inv X0. inv X2.
+    exact (bindIO (poke X X1) X0).
+  dependent destruction midx; simpl in *.
+    inv args. inv X0. inv X2. inv X3.
+    exact (bindIO (memcpy X X1 X0) X2).
+  dependent destruction midx; simpl in *.
+    inv args. inv X0. inv X2. inv X3.
+    exact (bindIO (memset X X1 X0) X2).
+  inversion midx.
+Defined.
+
+Corollary bind_If `{Monad f} : forall A B (k : A -> f B) b t e,
+  ((If b Then t Else e) >>= k) = If b Then t >>= k Else e >>= k.
+Proof. destruct b; reflexivity. Qed.
+
+Corollary fmap_If `{Functor f} : forall A B (k : A -> B) b t e,
+  fmap k (If b Then t Else e) = If b Then fmap k t Else fmap k e.
+Proof. destruct b; reflexivity. Qed.
+
+Corollary iter_If `{Functor f} : forall A (phi : f A -> A) b t e,
+  iter phi (If b Then t Else e) = If b Then iter phi t Else iter phi e.
+Proof. destruct b; reflexivity. Qed.
+
+Lemma ghcConsDSL :
+  { f : PS -> Word -> PS
+  & forall bs w, f bs w = ghcDenote (fst <$> projT1 (consDSL w) bs) }.
+Proof.
+  eexists.
+  intros.
+  unfold consDSL, ghcDenote, compose, comp.
+  symmetry.
+  simpl projT1.
+  do 6 rewrite fmap_If.
+  simpl.
+  do 3 setoid_rewrite iter_If.
+  simpl.
+  unfold If_Then_Else, compose, comp; simpl.
+  unfold solution_left, eq_rect_r, eq_rect.
+  simpl.
+  unfold simplification_heq.
+  unfold solution_right, eq_rect_r, eq_rect.
+  simpl.
+  unfold block.
+  simpl.
+  remember (eq_sym _) as E.
+  dependent destruction E.
+  simpl.
+  rewrite <- HeqE.
+  etransitivity.
+    simpl.
+    reflexivity.
+  rewrite !bindIO_returnIO.
+  reflexivity.
+Defined.
+
+Definition ghcConsDSL' := Eval simpl in projT1 ghcConsDSL.
+Print ghcConsDSL'.
 
 Theorem consDSL_correct : forall (r : Rep HeapSpec) (bs : PS) w,
   refine (buffer_cons r bs w)
@@ -337,73 +548,6 @@ Proof.
     autorewrite with monad laws; reflexivity.
   autorewrite with monad laws; reflexivity.
 Qed.
-
-Axiom IO : Type -> Type.
-
-Axiom fmapIO   : forall {a b : Type}, (a -> b) -> IO a -> IO b.
-Axiom bindIO   : forall {a b : Type}, IO a -> (a -> IO b) -> IO b.
-Axiom returnIO : forall {a : Type}, a -> IO a.
-Axiom joinIO   : forall {a : Type}, IO (IO a) -> IO a.
-
-Axiom bindIO_returnIO : forall {a b : Type} (f : a -> b) (x : IO a),
-  bindIO x (fun a => returnIO (f a)) = fmapIO f x.
-
-Axiom unsafeDupablePerformIO : forall {a : Type}, IO a -> a.
-
-Axiom malloc  : Size -> IO (Ptr Word).
-Axiom free    : Ptr Word -> IO ().
-Axiom realloc : Ptr Word -> Size -> IO (Ptr Word).
-Axiom peek    : Ptr Word -> IO Word.
-Axiom poke    : Ptr Word -> Word -> IO ().
-Axiom memcpy  : Ptr Word -> Ptr Word -> Size -> IO ().
-Axiom memset  : Ptr Word -> Size -> Word -> IO ().
-
-Definition ghcDenote {A : Type} : HeapDSL A -> A :=
-  let phi (c : HeapF (IO A)) :=
-    match c with
-    | Alloc len k             => bindIO (malloc (` len)) k
-    | Free_ addr x            => bindIO (free addr) (fun _ => x)
-    | Realloc addr len k      => bindIO (realloc addr (` len)) k
-    | Peek addr k             => bindIO (peek addr) k
-    | Poke addr w x           => bindIO (poke addr w) (fun _ => x)
-    | Memcpy addr addr2 len x => bindIO (memcpy addr addr2 len) (fun _ => x)
-    | Memset addr len w x     => bindIO (memset addr len w) (fun _ => x)
-    end in
-  unsafeDupablePerformIO \o iter phi \o fmap returnIO.
-
-Corollary bind_If `{Monad f} : forall A B (k : A -> f B) b t e,
-  ((If b Then t Else e) >>= k) = If b Then t >>= k Else e >>= k.
-Proof. destruct b; reflexivity. Qed.
-
-Corollary fmap_If `{Functor f} : forall A B (k : A -> B) b t e,
-  fmap k (If b Then t Else e) = If b Then fmap k t Else fmap k e.
-Proof. destruct b; reflexivity. Qed.
-
-Corollary iter_If `{Functor f} : forall A (phi : f A -> A) b t e,
-  iter phi (If b Then t Else e) = If b Then iter phi t Else iter phi e.
-Proof. destruct b; reflexivity. Qed.
-
-Lemma ghcConsDSL :
-  { f : PS -> Word -> PS
-  & forall bs w, f bs w = ghcDenote (fst <$> projT1 (consDSL w) bs) }.
-Proof.
-  eexists.
-  intros.
-  unfold consDSL, ghcDenote, compose, comp.
-  symmetry.
-  simpl projT1.
-  do 6 rewrite fmap_If.
-  etransitivity.
-    do 3 setoid_rewrite iter_If.
-    simpl.
-    unfold If_Then_Else, compose, comp; simpl.
-    reflexivity.
-  rewrite !bindIO_returnIO.
-  reflexivity.
-Defined.
-
-Definition ghcConsDSL' := Eval simpl in projT1 ghcConsDSL.
-Print ghcConsDSL'.
 
 End ByteStringFFI.
 
